minimize the Context API

Cslib/Languages/LambdaCalculus/LocallyNameless/Context.lean
@@ -17,85 +17,19 @@ Contexts as pairs of free variables and types.
 
 universe u v
 
-variable {Var : Type u} {Ty : Type v} [DecidableEq Var]
+variable {α : Type u} {β : Type v} [DecidableEq α]
 
-namespace LambdaCalculus.LocallyNameless
-
-/-- A typing context is a list of free variables and corresponding types. -/
-abbrev Context (Var : Type u) (Ty : Type v) := List ((_ : Var) × Ty)
-
-namespace Context
-
-open List
-
-/-- The domain of a context is the finite set of free variables it uses. -/
-@[simp, grind =]
-def dom (Γ : Context Var Ty) : Finset Var := Γ.keys.toFinset
-
-/-- A well-formed context. -/
-abbrev Ok : Context Var Ty → Prop := NodupKeys
-
-instance : HasWellFormed (Context Var Ty) :=
-  ⟨Ok⟩
-
-variable {Γ Δ : Context Var Ty}
-
-omit [DecidableEq Var] in
-@[grind _=_]
-theorem haswellformed_def : Γ✓ = Γ.NodupKeys := by rfl
-
-/-- Context membership implies membership in the domain. -/
-@[scoped grind →]
-theorem dom_mem (mem : ⟨x, σ⟩ ∈ Γ) : x ∈ Γ.dom := by
-  simp only [dom, mem_toFinset, keys]
-  grind
-
-/-- Context membership is preserved on permuting a context. -/
-theorem dom_perm_mem_iff (h : Γ.Perm Δ) {x : Var} : x ∈ Γ.dom ↔ x ∈ Δ.dom := by
-  induction h <;> simp_all only [dom, mem_toFinset, keys_cons, mem_cons] 
-  grind
-
-omit [DecidableEq Var] in
-/-- Context well-formedness is preserved on permuting a context. -/
-@[scoped grind →]
-theorem wf_perm (h : Γ.Perm Δ) : Γ✓ → Δ✓ := (List.perm_nodupKeys h).mp
-
-omit [DecidableEq Var] in
-/-- Context well-formedness is preserved on removing an element. -/
-@[scoped grind →]
-theorem wf_strengthen (ok : (Δ ++ ⟨x, σ⟩ :: Γ)✓) : (Δ ++ Γ)✓ := by
-  exact List.NodupKeys.sublist (by simp) ok
-
-@[simp, scoped grind]
-def map_val (f : Ty → Ty) (Γ : Context Var Ty) : Context Var Ty := 
-  Γ.map (fun ⟨var,ty⟩ => ⟨var,f ty⟩)
-
-theorem map_val_ok (ok : Γ✓) (f : Ty → Ty) : (Γ.map_val f)✓ := by
-  induction Γ
-  case nil => grind
-  case cons hd tl ih =>
-    cases ok
-    constructor <;> grind
-
-lemma map_val_mem (mem : σ ∈ Γ.dlookup x) (f) : f σ ∈ (Γ.map_val f).dlookup x := by
-  induction Γ
-  case nil => simp at mem
-  case cons hd tl ih =>
-    let ⟨x',σ'⟩ := hd
-    by_cases h : x = x'
-    · subst h
-      simp_all [map_val]
-    · grind [List.dlookup_cons_ne]
-
-end LambdaCalculus.LocallyNameless.Context
-
+-- TODO: These are pieces of API that cannot be directly automated by adding `grind` attributes to
+-- `Mathlib.Data.List.Sigma`. We should consider upstreaming them to Mathlib.
 namespace List
 
-variable {α : Type u} {β : α → Type v} 
+variable {β : α → Type v} {Γ Δ : List (Sigma β)}
 
-variable [DecidableEq α]
+/-- List permutation preserves keys. -/
+theorem perm_keys (h : Γ.Perm Δ) : x ∈ Γ.keys ↔ x ∈ Δ.keys := by
+  induction h <;> grind [keys_cons]
 
--- TODO: this should upstream to Mathlib
+/-- Sublists without deuplicate keys preserve lookups. -/
 @[grind]
 theorem sublist_dlookup (l₁ l₂ : List (Sigma β)) (nd₁ : l₁.NodupKeys) (nd₂ : l₂.NodupKeys)
     (s : l₁ <+ l₂) (mem : b ∈ l₁.dlookup a) : b ∈ l₂.dlookup a := by
@@ -115,6 +49,7 @@ theorem sublist_dlookup (l₁ l₂ : List (Sigma β)) (nd₁ : l₁.NodupKeys) (
       exact mem
     · simp_all
 
+/-- A lookup in appended lists must appear in one of the lists. -/
 theorem dlookup_append_mem (l₁ l₂ : List (Sigma β)) (mem : b ∈ (l₁ ++ l₂).dlookup a) : 
     b ∈ l₁.dlookup a ∨ b ∈ l₂.dlookup a := by
   rw [List.dlookup_append l₁ l₂ a] at mem
@@ -122,3 +57,67 @@ theorem dlookup_append_mem (l₁ l₂ : List (Sigma β)) (mem : b ∈ (l₁ ++ l
   grind
 
 end List
+
+namespace LambdaCalculus.LocallyNameless
+
+/-- A typing context is a list of free variables and corresponding types. -/
+abbrev Context (α : Type u) (β : Type v) := List ((_ : α) × β)
+
+namespace Context
+
+-- we would like grind to see through certain notations
+attribute [scoped grind] Option.mem_def
+attribute [scoped grind _=_] List.append_eq
+attribute [scoped grind] List.Nodup
+attribute [scoped grind] List.NodupKeys
+
+-- we would like grind to treat list and finset membership the same
+attribute [scoped grind] List.mem_toFinset
+
+-- otherwise, we mostly reuse existing API in `Mathlib.Data.List.Sigma`
+attribute [scoped grind] List.keys
+attribute [scoped grind →] List.mem_keys_of_mem
+attribute [scoped grind] List.dlookup_isSome
+attribute [scoped grind] List.perm_nodupKeys
+attribute [scoped grind →] List.perm_nodupKeys
+attribute [scoped grind →] List.Perm.symm
+
+/-- The domain of a context is the finite set of free variables it uses. -/
+@[simp, scoped grind =]
+def dom (Γ : Context α β) : Finset α := Γ.keys.toFinset
+
+/-- A well-formed context has no duplicate keys. -/
+instance : HasWellFormed (Context α β) :=
+  ⟨List.NodupKeys⟩
+
+omit [DecidableEq α] in
+@[scoped grind _=_]
+theorem haswellformed_def (Γ : Context α β) : Γ✓ = Γ.NodupKeys := by rfl
+
+variable {Γ Δ : Context α β}
+
+/-- A mapping of values within a context. -/
+@[simp, scoped grind]
+def map_val (f : β → β) (Γ : Context α β) : Context α β := 
+  Γ.map (fun ⟨var,ty⟩ => ⟨var,f ty⟩)
+
+/-- A mapping of values preserves non-duplication of keys. -/
+theorem map_val_ok (ok : Γ✓) (f : β → β) : (Γ.map_val f)✓ := by
+  induction Γ
+  case nil => grind
+  case cons hd tl ih =>
+    cases ok
+    constructor <;> grind
+
+/-- A mapping of values preserves lookups. -/
+lemma map_val_mem (mem : σ ∈ Γ.dlookup x) (f) : f σ ∈ (Γ.map_val f).dlookup x := by
+  induction Γ
+  case nil => simp at mem
+  case cons hd tl ih =>
+    let ⟨x',σ'⟩ := hd
+    by_cases h : x = x'
+    · subst h
+      simp_all [map_val]
+    · grind [List.dlookup_cons_ne]
+
+end LambdaCalculus.LocallyNameless.Context
